src/Lean/Meta/Basic.lean
@@ -489,7 +489,6 @@ structure Context where
    This is not a great solution, but a proper solution would require a more sophisticased caching mechanism.
   -/
   inTypeClassResolution : Bool := false
-  localDfEqs : List Expr := []
   fuel : Nat := 5
 
 /--
@@ -1785,9 +1784,6 @@ caller ensure the local instances are also properly updated.
 -/
 def withLCtx' (lctx : LocalContext) : n α → n α :=
   mapMetaM <| withReader (fun ctx => { ctx with lctx })
-
-def withLocalDfEq (e : Expr) : n α → n α :=
-  mapMetaM <| withReader (fun c => {c with localDfEqs := c.localDfEqs ++ [e]})
 
 /--
 Runs `k` in a local environment with the `fvarIds` erased.
